lib/prelude/consistency.bpl
@@ -10,6 +10,8 @@
  * Exported declarations
  */
 
+ type Vis = [Invoc] Set;
+
 // hb(x, y) : x happens-before y.
 // We assume there exists such a function, given by the client program
 function hb(x: Invoc, y: Invoc): bool;
@@ -19,4 +21,12 @@ axiom (forall n: Invoc :: !hb(n, n));
 var {:layer 1,2} lin: Seq;
 
 // A map from invocations to the set of prior invocations visible to them
-var {:layer 1,2} vis: [Invoc] Set;
+var {:layer 1,2} vis: Vis;
+
+function {:inline} Consistency.complete(lin: Seq, vis: Vis, this: Invoc): bool {
+  vis[this] == Set.ofSeq(lin)
+}
+
+function {:inline} Consistency.monotonic(lin: Seq, vis: Vis, this: Invoc): bool {
+  (forall i: Invoc :: hb(i, this) ==> Set.subset(vis[i], vis[this]))
+}
